src/ext_traversal/ExtTraversalCounting.v
@@ -7,6 +7,7 @@ Require Import AuxRel2.
 Require Import TraversalConfig.
 Require Import Traversal.
 Require Import ExtTraversalConfig.
+Require Import ExtTraversal.
 Require Import ExtSimTraversal.
 Require Import ExtSimTraversalProperties.
 
